iptables-semantics/IptablesSemantics/iptables/syntax.lean
@@ -1,4 +1,4 @@
-namespace Firewall
+namespace Iptables
 
 /-- Actions -/
 inductive Action
@@ -12,7 +12,7 @@ inductive Action
 | Empty
 | Unknown
 
-end Firewall
+end Iptables
 
 /--Match expressions-/
 inductive MatchExpr (A : Type) -- polimorphic type A, works for any type A
@@ -22,10 +22,10 @@ inductive MatchExpr (A : Type) -- polimorphic type A, works for any type A
 | MatchAny -- an always true expression
 
 /--Builds Or via De Morgan-/
-def Firewall.matchOr {A} (m1 m2 : MatchExpr A) : MatchExpr A
+def Iptables.matchOr {A} (m1 m2 : MatchExpr A) : MatchExpr A
   := MatchExpr.MatchNot (MatchExpr.MatchAnd (MatchExpr.MatchNot m1) (MatchExpr.MatchNot m2))
 
 /--A firewall rule consists of a match experssion and an action-/
-structure Firewall.Rule (A : Type) where -- given A, define a type Rule A
+structure Iptables.Rule (A : Type) where
           matchExpr : MatchExpr A
           action : Action
