iptables-semantics/IptablesSemantics/iptables/decision_state.lean
@@ -1,4 +1,4 @@
-namespace Firewall
+namespace Iptables
 
 /-- Final decision -/
 inductive FinalDecision
@@ -10,4 +10,4 @@ inductive ProcessingDecision
   | undecided
   | decision (d : FinalDecision) --take an argument d of type Final Decision and return as Processing Decision
 
-end Firewall
+end Iptables
