iptables-semantics/IptablesSemantics/nftables/nf_iptables_equiv.lean
@@ -1,0 +1,773 @@
+import IptablesSemantics.nftables.nf_syntax
+import IptablesSemantics.nftables.nf_semantics
+import IptablesSemantics.iptables.semantics
+import Mathlib.Tactic
+import Hammer
+open Iptables
+open Nftables
+
+inductive simulation : ProcessingDecision -> Registers -> Prop where
+  | undecided :
+    simulation ProcessingDecision.undecided
+    { verdict := Verdict.NFT_CONTINUE, destination_chain := none}
+  | allow :
+    simulation (ProcessingDecision.decision FinalDecision.allow)
+    { verdict := Verdict.NFT_ACCEPT, destination_chain := none}
+  | deny :
+    simulation (ProcessingDecision.decision FinalDecision.deny)
+    { verdict := Verdict.NFT_DROP, destination_chain := none }
+
+/-- The iptables initial state (undecided) and nftables initial state (initial_register)
+   satisfy the simulation relation -/
+theorem simul_initial : simulation ProcessingDecision.undecided initial_register := by
+  unfold initial_register
+  exact simulation.undecided
+
+/-- Determinism for simulation relation  each ProcessingDecision maps exactly one Registers state
+-/
+theorem simRel_deterministic : ∀ (pd : ProcessingDecision) (r1 r2 : Registers),
+                              simulation pd r1 -> simulation pd r2 -> r1 = r2 := by
+  intro pd r1 r2 h1 h2
+  cases h1 <;>
+  cases h2 <;>
+  rfl
+
+/--Totality for simulation relation = rach iptables state has a corresponding nftables state.
+   -/
+theorem simrel_total : ∀ (pd : ProcessingDecision), ∃ (r : Registers),
+simulation pd r := by
+  intro pd
+  cases pd with
+  | undecided =>
+    use { verdict := Verdict.NFT_CONTINUE, destination_chain := none }
+    apply simulation.undecided
+  | decision d =>
+    cases d with
+    | allow =>
+      use { verdict := Verdict.NFT_ACCEPT, destination_chain := none }
+      apply simulation.allow
+    | deny =>
+      use { verdict := Verdict.NFT_DROP, destination_chain := none }
+      apply simulation.deny
+
+/-- ProcessingDecision to Registers.
+   -/
+def state_to_regs : ProcessingDecision -> Registers
+  | ProcessingDecision.undecided =>
+    {verdict := Verdict.NFT_CONTINUE, destination_chain := none}
+  | ProcessingDecision.decision Iptables.FinalDecision.allow =>
+    {verdict := Verdict.NFT_ACCEPT, destination_chain := none}
+  | ProcessingDecision.decision Iptables.FinalDecision.deny =>
+    {verdict := Verdict.NFT_DROP, destination_chain := none}
+
+/-- state_to_regs is consistent with simulation -/
+theorem state_to_regs_simrel : ∀ (pd : ProcessingDecision), simulation pd (state_to_regs pd) := by
+  intro pd
+  cases pd with
+  | undecided => exact simulation.undecided
+  | decision d =>
+    cases d with
+    | allow => exact simulation.allow
+    | deny => exact simulation.deny
+
+/-- state_to_regs undecided equals initial_register-/
+theorem state_to_regs_undecided :
+  state_to_regs ProcessingDecision.undecided = initial_register :=
+  rfl
+
+def translate_match {A : Type} : MatchExpr A -> Expression A
+  | m => Expression.Comparison m
+
+/-- translate iptables Action to nftables Statement-/
+def action_to_statement : Action -> Statement
+  | Action.Accept => Statement.Accept
+  | Action.Drop => Statement.Drop
+  | Action.Reject => Statement.Drop
+  | Action.Call chain => Statement.Jump chain
+  | Action.Goto chain => Statement.Goto chain
+  | Action.Return => Statement.Return
+  | Action.Log => Statement.Continue
+  | Action.Empty => Statement.Continue
+  | Action.Unknown => Statement.Continue
+
+/--Rule translation: convert iptables rule to nftables rule
+   The match expression becomes a single comparison expression,
+   and the action becomes a statement -/
+def rule_translation {A : Type} : Iptables.Rule A -> Nftables.Rule A
+  | {matchExpr := m, action := a} =>
+    { expressions := [translate_match m],
+      statement := action_to_statement a }
+
+/--Ruleset translation-/
+def ruleset_translation {A : Type} : List (Iptables.Rule A) -> List (Nftables.Rule A)
+  | [] => []
+  | r :: rs => rule_translation r :: ruleset_translation rs
+
+/--Translate a ruleset map from iptables to nftables-/
+def translate_ruleset {A : Type} (Γ : Ruleset A) : NfRuleset A :=
+  fun chain => Option.map ruleset_translation (Γ chain)
+
+
+/-- If the iptables match expression m succeeds on packet p,
+then the translated nftables expression list [ translation (m) ] also succeds.-/
+lemma l1_match {A P : Type} (γ : Matcher A P) (p : P) (m : MatchExpr A) (regs : Registers)
+  (hmatch : matchExpression γ m p = true) :
+  expressions_match γ p [translate_match m] regs ExprListEval.elist_match := by
+
+  unfold translate_match
+  apply expressions_match.cont
+  -- ⊢ expression_evaluation γ p (have m := m; Expression.Comparison m false) regs ?regs1
+  -- comparison_true applies with matchExp = true
+  case a => exact expression_evaluation.comparison_true hmatch
+  -- ⊢ { verdict := Verdict.NFT_CONTINUE, destination_chain := regs.destination_chain }.verdict = Verdict.NFT_CONTINUE
+  -- after comparison_true, Verdict.NFT_CONTINUE by def
+  case a => rfl
+  --⊢ expressions_match γ p [] { verdict := Verdict.NFT_CONTINUE, destination_chain := regs.destination_chain } ExprListEval.elist_match
+  case a => exact expressions_match.empty
+
+/--If the iptables match expression m doesn’t succeed on packet p,
+then the translated nftables expression list [ translation (m) ] also doesn’t succeed. -/
+lemma l1_nomatch {A P : Type}
+    (γ : Matcher A P) (p : P) (m : MatchExpr A) (regs : Registers)
+    (hmatch : matchExpression γ m p = false) :
+    expressions_match γ p [translate_match m] regs ExprListEval.elist_nomatch := by
+
+  unfold translate_match
+  apply expressions_match.fail
+  -- ⊢ expression_evaluation γ p (have m := m; Expression.Comparison m false) regs ?regs1
+  case a => exact expression_evaluation.comparison_false hmatch
+  -- hmatch : matchExpression γ m p = false
+  -- ⊢ matchExpression γ m p = false
+  case a => rfl
+
+/-- Base case for forward simulation.
+Accept in iptables => Accept in nftables (if an iptables ule with Accept
+matches a packet, then the translated nftables rule
+gives an equivalent NFT_ACCEPT verdict.)
+-/
+theorem accept_equivalence {A P : Type} (Γ : Ruleset A) (γ : Matcher A P)(m : MatchExpr A)  (p : P)
+
+(hyp_match : matchExpression γ m p = true) :
+
+∃ regs, ruleset_evaluation (translate_ruleset Γ) γ p
+(ruleset_translation [{ matchExpr := m, action := Action.Accept }]) initial_register regs
+∧ simulation (ProcessingDecision.decision FinalDecision.allow) regs := by
+
+  use { initial_register with verdict := Verdict.NFT_ACCEPT, destination_chain := none }
+  apply And.intro
+  case h.left =>
+    apply ruleset_evaluation.accept
+    · rfl
+    · apply rule_evaluation.elist_match
+      exact l1_match γ p m initial_register hyp_match
+    · rfl
+  case h.right =>
+    exact simulation.allow
+
+
+theorem drop_rej_equivalence {A P : Type} (Γ : Ruleset A) (γ : Matcher A P) (p : P)
+(m : MatchExpr A) (hyp_match : matchExpression γ m p = true) :
+∃ regs, ruleset_evaluation (translate_ruleset Γ) γ p
+(ruleset_translation [{ matchExpr := m, action := Action.Drop }])
+initial_register regs
+∧ simulation (ProcessingDecision.decision FinalDecision.deny) regs := by
+  use { initial_register with verdict := Verdict.NFT_DROP, destination_chain := none }
+  apply And.intro
+  case h.left =>
+    apply ruleset_evaluation.drop
+    · rfl
+    · apply rule_evaluation.elist_match
+      exact l1_match γ p m initial_register hyp_match
+    · rfl
+  case h.right =>
+    exact simulation.deny
+
+
+/--If the iptables rule does not match the packet, then the translated nftables
+rule also does not match, so the rule is skipped and the verdict says NFT_CONTINUE-/
+theorem noMatch_equivalence {A P : Type} (Γ : Ruleset A) (γ : Matcher A P) (p : P)
+(m : MatchExpr A) (a : Action) (hyp_match : matchExpression γ m p = false) :
+∃ regs, ruleset_evaluation (translate_ruleset Γ) γ p (ruleset_translation [{ matchExpr := m, action := a }]) initial_register regs
+∧ simulation ProcessingDecision.undecided regs := by
+  -- ⊢ ∃ regs, ruleset_evaluation (translate_ruleset Γ) γ p (ruleset_translation [{ matchExpr := m, action := a }]) initial_register regs ∧
+  -- simulation ProcessingDecision.undecided regs
+  -- the witness is Continue for noMatch
+  use { initial_register with verdict := Verdict.NFT_CONTINUE, destination_chain := none }
+  apply And.intro
+  -- h.left :⊢ ruleset_evaluation (translate_ruleset Γ) γ p (ruleset_translation [{ matchExpr := m, action := a }]) initial_register
+  --(let __src := initial_register;
+  --{ verdict := Verdict.NFT_CONTINUE, destination_chain := __src.destination_chain })
+  -- h.right: ⊢ simulation ProcessingDecision.undecided
+  --(let __src := initial_register;
+  -- { verdict := Verdict.NFT_CONTINUE, destination_chain := __src.destination_chain })
+  case h.left =>
+    apply ruleset_evaluation.nf_continue
+    -- ⊢ initial_register.verdict = Verdict.NFT_CONTINUE
+    · rfl
+    -- ⊢ rule_evaluation (translate_ruleset Γ) γ p (rule_translation { matchExpr := m, action := a }) initial_register ?regs1
+    · apply rule_evaluation.elist_nomatch
+      exact l1_nomatch γ p m initial_register hyp_match
+    -- ⊢ { verdict := Verdict.NFT_CONTINUE, destination_chain := initial_register.destination_chain }.verdict =
+    -- Verdict.NFT_CONTINUE
+    · rfl
+    -- ⊢ ruleset_evaluation (translate_ruleset Γ) γ p (ruleset_translation [])
+    -- { verdict := Verdict.NFT_CONTINUE, destination_chain := initial_register.destination_chain }
+    -- (let __src := initial_register;
+    -- { verdict := Verdict.NFT_CONTINUE, destination_chain := __src.destination_chain })
+    · exact ruleset_evaluation.skip
+  case h.right =>
+    exact simulation.undecided
+
+theorem log_equivalence {A P : Type} (Γ : Ruleset A) (γ : Matcher A P) (p : P)
+(m : MatchExpr A) (hyp_match : matchExpression γ m p = true) :
+∃ regs2,
+  ruleset_evaluation (translate_ruleset Γ) γ p
+    (ruleset_translation [{ matchExpr := m, action := Action.Log }])
+    initial_register regs2
+  ∧ simulation ProcessingDecision.undecided regs2 := by
+  -- ⊢ ∃ regs2,
+  -- ruleset_evaluation (translate_ruleset Γ) γ p (ruleset_translation [{ matchExpr := m, action := Action.Log }])
+  -- initial_register regs2 ∧
+  -- simulation ProcessingDecision.undecided regs2
+  use { initial_register with verdict := Verdict.NFT_CONTINUE, destination_chain := none }
+  apply And.intro
+  case h.left =>
+    apply ruleset_evaluation.nf_continue
+    · rfl
+    · apply rule_evaluation.elist_match
+      exact l1_match γ p m initial_register hyp_match
+    · rfl
+    · exact ruleset_evaluation.skip
+  case h.right =>
+    exact simulation.undecided
+
+theorem empty_equivalence {A P : Type} (Γ : Ruleset A) (γ : Matcher A P) (p : P)
+(m : MatchExpr A) (hyp_match : matchExpression γ m p = true) :
+∃ regs2, ruleset_evaluation (translate_ruleset Γ) γ p (ruleset_translation [{ matchExpr := m, action := Action.Empty }])
+initial_register regs2 ∧ simulation ProcessingDecision.undecided regs2 := by
+  use { initial_register with verdict := Verdict.NFT_CONTINUE, destination_chain := none }
+  apply And.intro
+  case h.left =>
+    apply ruleset_evaluation.nf_continue
+    · rfl
+    · apply rule_evaluation.elist_match
+      exact l1_match γ p m initial_register hyp_match
+    · rfl
+    · exact ruleset_evaluation.skip
+  case h.right =>
+    exact simulation.undecided
+
+/- This is used in seq_equivalence_full (also I used it in call_return for rs1 ++ Return ++ rs2) to prove that translating rs1 ++ rs2 works.
+    Evaluating a concatenation is the same evaluating sequentially with CONTINUE
+    Given separate derivations for rs1 and rs2, construct a combined derivation
+    for rs1++rs2-/
+lemma ruleset_evaluation_append_continue
+  -- rs1 evaluates regs1 -> regs_mid with Continue
+  (H1 : ruleset_evaluation Γ γ p rs1 regs1 regs_mid)
+  (hcont : regs_mid.verdict = Verdict.NFT_CONTINUE)
+  -- rs2 evaluates regs2_mid -> regs12
+  (H2 : ruleset_evaluation Γ γ p rs2 regs_mid regs2) :
+  -- (rs1 ++ rs2) evaluates regs1 -> regs2
+  ruleset_evaluation Γ γ p (rs1 ++ rs2) regs1 regs2 := by
+  -- ⊢ ruleset_evaluation Γ γ p (rs1 ++ rs2) regs1 regs2
+  -- ruleset_evuation is an inductive relation
+  induction H1 generalizing regs2 with
+  | skip => simpa using H2
+  | nf_continue hcont_in rule_eval verdict_cont ruleset_eval ih =>
+    have tail := ih hcont H2
+    simpa using ruleset_evaluation.nf_continue hcont_in rule_eval verdict_cont tail
+  -- contradiction for accept, drop, stolen, nf_return (used hammer for those)
+  | accept => simp_all only [reduceCtorEq]
+  | drop _ _ hv => simp_all only [reduceCtorEq]
+  | stolen _ _ hv => simp_all only [reduceCtorEq]
+  | nf_return _ _ hv =>  simp_all only [reduceCtorEq]
+  | jump hcont_in hrule hvjump hdest hchain hchain_eval hrs_eval _ ih_rs =>
+    have tail := ih_rs hcont H2
+    simpa using ruleset_evaluation.jump hcont_in hrule hvjump hdest hchain hchain_eval tail
+  | goto =>
+    -- hvgoto says verdict = NFT_GOTO
+    -- hcont says verdict = NFT_CONTINUE
+    simp_all
+    sorry
+  -- goto is a tail-call; can't append after it (used hammer)
+  | terminal ht => simp_all only [reduceCtorEq, or_self]
+
+/-- If rs1 produces a terminal verdict, then rs1 ++ rs2 also produces the same result -/
+lemma ruleset_evaluation_append_terminal {A P : Type} {Γ : NfRuleset A} {γ : Matcher A P} {p : P}
+    {rs1 rs2 : List (Nftables.Rule A)} {regs1 regs_mid : Registers}
+    (h1 : ruleset_evaluation Γ γ p rs1 regs1 regs_mid)
+    (hterminal : regs_mid.verdict = Verdict.NFT_ACCEPT ∨ regs_mid.verdict = Verdict.NFT_DROP) :
+    ruleset_evaluation Γ γ p (rs1 ++ rs2) regs1 regs_mid := by
+  induction h1 with
+  | skip => simp; exact ruleset_evaluation.terminal hterminal
+  | nf_continue hcont_in rule_eval verdict_cont _ ih =>
+    simpa using ruleset_evaluation.nf_continue hcont_in rule_eval verdict_cont (ih hterminal)
+  | accept hcont hr hv => simpa using ruleset_evaluation.accept hcont hr hv
+  | drop hcont hr hv => simpa using ruleset_evaluation.drop hcont hr hv
+  | stolen hcont hr hv => simp_all  -- STOLEN is not ACCEPT or DROP
+  | nf_return hcont hr hv => simp_all  -- RETURN is not ACCEPT or DROP
+  | jump hcont hr hv hd hc hchain hrs _ ih_rs =>
+    simpa using ruleset_evaluation.jump hcont hr hv hd hc hchain (ih_rs hterminal)
+  | goto hcont hr hv hd hc hchain _ =>
+    simp only [List.cons_append]
+    exact ruleset_evaluation.goto hcont hr hv hd hc hchain
+  | terminal ht => exact ruleset_evaluation.terminal ht
+
+/-- T(rs1 ++ rs2) = T(rs1) ++ T(rs2)  -/
+lemma rs_homomorphism (rs1 rs2 : List (Iptables.Rule A)) :
+    ruleset_translation (rs1 ++ rs2) =
+    ruleset_translation rs1 ++ ruleset_translation rs2 := by
+  induction rs1 with
+  | nil => rfl
+  | cons r rs h =>
+    simp only[ruleset_translation, List.cons_append, h]
+
+/-- simulation undecided implies NFT_CONTINUE verdict -/
+lemma simrel_undecided_continue {regs : Registers}
+    (h : simulation ProcessingDecision.undecided regs) :
+    regs.verdict = Verdict.NFT_CONTINUE := by
+  cases h
+  rfl
+
+-- the translated nftables evaluation of rs starting from regs gives
+-- a state regs1 related to iptables decision t
+def nf_eval_produces {A P : Type} (Γ : Ruleset A) (γ : Matcher A P) (p : P)
+    (rs : List (Iptables.Rule A)) (regs_in : Registers) (t_out : ProcessingDecision) : Prop :=
+  ∃ regs_out, ruleset_evaluation (translate_ruleset Γ) γ p (ruleset_translation rs) regs_in regs_out
+    ∧ simulation t_out regs_out
+
+/- If you run rs1 and rs2 sequentially in iptables, the translated
+nftables gives the same results. -/
+theorem seq_equivalence_full {A P : Type} (Γ : Ruleset A) (γ : Matcher A P) (p : P)
+(rs1 rs2 : List (Iptables.Rule A)) (t : ProcessingDecision)
+
+/- For any regs_in that's undecided -> evaluating rs1 stays undecided -/
+(H1 : ∀ regs_in, simulation ProcessingDecision.undecided regs_in ->
+  nf_eval_produces Γ γ p rs1 regs_in ProcessingDecision.undecided)
+
+/- For any regs_mid that's undecided -> evaluating rs2 gives decision t -/
+(H2 : ∀ regs_mid, simulation ProcessingDecision.undecided regs_mid ->
+  nf_eval_produces Γ γ p rs2 regs_mid t)
+
+(regs : Registers) (simrel : simulation ProcessingDecision.undecided regs) :
+
+/- There exist some regs_out, such that evaluating the translated rs1 ++ rs2
+   from regs gives regs_out, and it satisfies the relation with decision t -/
+∃ regs_out, ruleset_evaluation (translate_ruleset Γ) γ p (ruleset_translation (rs1 ++ rs2)) regs regs_out
+∧ simulation t regs_out := by
+  -- ⊢ ∃ regs_out,
+  -- ruleset_evaluation (translate_ruleset Γ) γ p (ruleset_translation (rs1 ++ rs2)) regs regs_out
+  -- ∧ simulation t regs_out
+  unfold nf_eval_produces at H1
+  unfold nf_eval_produces at H2
+  have ⟨regs_mid, rs_eval1, int_sim⟩ := H1 regs simrel
+  have ⟨regs_out, rs_eval2, fin_sim⟩ := H2 regs_mid int_sim
+  have mid_verdict : regs_mid.verdict = Verdict.NFT_CONTINUE := simrel_undecided_continue int_sim
+  rw [rs_homomorphism]
+  use regs_out
+  constructor
+  case h.left => exact ruleset_evaluation_append_continue rs_eval1 mid_verdict rs_eval2
+  case h.right => exact fin_sim
+
+
+theorem skip_equivalence {A P : Type} (Γ : Ruleset A) (γ : Matcher A P) (p : P)
+  (t : ProcessingDecision) (regs : Registers) (sim : simulation t regs) :
+  ∃ regs', ruleset_evaluation (translate_ruleset Γ) γ p (ruleset_translation []) regs regs'
+  ∧ simulation t regs' := by
+  simp [ruleset_translation]
+  exact ⟨regs, ruleset_evaluation.skip, sim⟩
+
+theorem decision_equivalence {A P : Type} (Γ : Ruleset A) (γ : Matcher A P) (p : P)
+    (rs : List (Iptables.Rule A)) (X : Iptables.FinalDecision) (regs : Registers)
+    (sim : simulation (ProcessingDecision.decision X) regs) :
+    ∃ regs', ruleset_evaluation (translate_ruleset Γ) γ p (ruleset_translation rs) regs regs'
+    ∧ simulation (ProcessingDecision.decision X) regs' := by
+    have terminal : regs.verdict = Verdict.NFT_ACCEPT ∨ regs.verdict = Verdict.NFT_DROP := by
+      cases sim with
+      | allow =>
+        left
+        rfl
+      | deny =>
+        right
+        rfl
+    exact ⟨regs, ruleset_evaluation.terminal terminal, sim⟩
+
+
+/--If an iptables Call rule's match expression succeds on a packet,
+then the translated nftables rule evaluates successfullt,
+producing the result of an applying a Jump statement-/
+lemma call_rule_eval {A P : Type} (Γ : Ruleset A) (γ : Matcher A P) (p : P)
+(m : MatchExpr A) (chain : String) (hyp_match : matchExpression γ m p = true) :
+rule_evaluation (translate_ruleset Γ) γ p (rule_translation { matchExpr := m, action := Action.Call chain })
+initial_register (apply_statement (Statement.Jump chain) initial_register) := by
+-- l1_match : iptables match success -> nftables expressions match
+-- rule_evaluation.elist_match: expressions match -> rule evaluates
+  exact rule_evaluation.elist_match (l1_match γ p m initial_register hyp_match)
+
+lemma return_rule_eval {A P : Type} (Γ : Ruleset A) (γ : Matcher A P) (p : P)
+    (m : MatchExpr A) (regs : Registers) (hyp_match : matchExpression γ m p = true) :
+    rule_evaluation (translate_ruleset Γ) γ p
+      (rule_translation {matchExpr := m, action := Action.Return})
+      regs (apply_statement Statement.Return regs) := by
+  exact rule_evaluation.elist_match (l1_match γ p m regs hyp_match)
+
+/-- If iptables calls a chain and that chain hits a Return, then the
+  nftables translation produces undecided.
+
+  Jump logic (reminder):
+  - rules eval before call in main chain
+  - hit Call chain -> jump into the called chain
+  -- evaluate rs1 (stay undecided)
+  - hit Return and exit the called chain
+  -- rs2 is never reached
+  -- back to the main chain -/
+theorem call_return_equivalence {A P : Type} (Γ : Ruleset A) (γ : Matcher A P) (p : P)
+(m : MatchExpr A) (chain : String)
+
+(rs1 : List (Iptables.Rule A)) (m1 : MatchExpr A) (rs2 : List (Iptables.Rule A))
+-- the call rule in the main chain
+(hyp_match : matchExpression γ m p = true)
+
+-- rs1: rules before return
+-- rs2: rules after return (never executed)
+-- the called chain is split into: rs1 ++ [Return rule with m'] ++ rs2
+(hyp_chain : Γ chain = some (rs1 ++ [{ matchExpr := m1, action := Action.Return }] ++ rs2))
+-- the return rule in the main chain (proof that it fires)
+(hyp_match1 : matchExpression γ m1 p = true)
+
+-- assumption that rs1 preserves undecided decision
+(IH_rs1 : ∀ regs_in, simulation ProcessingDecision.undecided regs_in ->
+    nf_eval_produces Γ γ p rs1 regs_in ProcessingDecision.undecided) :
+
+--  call chain (which contains rs1 + Return + rs2 produces undecided)
+nf_eval_produces Γ γ p  [{ matchExpr := m, action := Action.Call chain }]
+initial_register ProcessingDecision.undecided := by
+  -- the Call rule translates correctly
+  have h_rule := call_rule_eval Γ γ p m chain hyp_match
+  -- need the proof that the rule fires
+  -- need proof that the chain evaluates
+  -- rs1 ++ [Return rule] ++ rs2
+  -- proof of how jump converts return -> continue
+  -- rs1 evaluates from initial_register to regs_int, staying in undecided
+  have ⟨regs_int, rs_eval1, sim_int⟩ := IH_rs1 initial_register simulation.undecided
+
+  -- registers after evaluating es1
+  have regs_mid : regs_int.verdict = Verdict.NFT_CONTINUE := simrel_undecided_continue sim_int
+
+  -- return rule fires from regs_int
+  have rule_return := return_rule_eval Γ γ p m1 regs_int hyp_match1
+
+  -- registers after return rule
+  let regs_return := apply_statement Statement.Return regs_int
+  have regs_return_pf : regs_return.verdict = Verdict.NFT_RETURN :=
+     -- ⊢ regs_return.verdict = Verdict.NFT_RETURN
+  rfl
+
+  -- [Return] ++ rs2 evaluates from regs_int to regs_return, rs2 is skipped
+  have ret_rs2 : ruleset_evaluation (translate_ruleset Γ) γ p
+    (rule_translation {matchExpr := m1, action := Action.Return} :: ruleset_translation rs2)
+    regs_int regs_return := by
+    -- ⊢ ruleset_evaluation (translate_ruleset Γ) γ p
+    -- (rule_translation { matchExpr := m1, action := Action.Return }
+    -- :: ruleset_translation rs2) regs_int regs_return
+    exact ruleset_evaluation.nf_return regs_mid rule_return regs_return_pf
+
+  -- rs1 ++ [Return] ++ rs2
+  have final_eval : ruleset_evaluation (translate_ruleset Γ) γ p
+    (ruleset_translation (rs1 ++ [{matchExpr := m1, action := Action.Return}] ++ rs2))
+    initial_register regs_return := by
+  -- ⊢ ruleset_evaluation (translate_ruleset Γ) γ p
+  -- (ruleset_translation (rs1 ++ [{ matchExpr := m1, action := Action.Return }] ++ rs2)) initial_register regs_return
+    repeat rw [rs_homomorphism]
+  -- ⊢ ruleset_evaluation (translate_ruleset Γ) γ p
+  -- (ruleset_translation rs1 ++ ruleset_translation [{ matchExpr := m1, action := Action.Return }] ++
+  -- ruleset_translation rs2)
+  -- initial_register regs_return
+
+  -- List.append_assoc - lemma
+  -- @[simp]
+  -- theorem List.append_assoc{α : Type u} (as bs cs : List α) :
+  -- as ++ bs ++ cs = as ++ (bs ++ cs)
+    simp [List.append_assoc]
+  -- ⊢ ruleset_evaluation (translate_ruleset Γ) γ p
+  --(ruleset_translation rs1 ++
+  -- (ruleset_translation [{ matchExpr := m1, action := Action.Return }] ++ ruleset_translation rs2))
+  -- initial_register regs_return
+    apply ruleset_evaluation_append_continue
+    --⊢ H1: ruleset_evaluation (translate_ruleset Γ) γ p (ruleset_translation rs1) initial_register ?regs_mid
+    -- hcont: ⊢ Registers.verdict ?regs_mid = Verdict.NFT_CONTINUE
+    -- H2: ⊢ ruleset_evaluation (translate_ruleset Γ) γ p
+    -- regs_mid : ⊢ Registers
+    case H1 =>
+      exact rs_eval1
+    case hcont =>
+      exact regs_mid
+    case H2 =>
+       exact ret_rs2
+
+    -- jump statement regs
+  let regs1 := apply_statement (Statement.Jump chain) initial_register
+  have jump_regs : regs1.verdict = Verdict.NFT_JUMP := by
+    exact rfl
+  have jump_dest_chain : regs1.destination_chain = some chain := by
+      exact rfl
+
+  have chain_lookup : (translate_ruleset Γ) chain = some
+   (ruleset_translation (rs1 ++ [{ matchExpr := m1, action := Action.Return}] ++ rs2)) := by
+  -- ⊢ translate_ruleset Γ chain = some (ruleset_translation (rs1 ++ [{ matchExpr := m1, action := Action.Return }] ++ rs2))
+    unfold translate_ruleset
+  -- ⊢ Option.map ruleset_translation (Γ chain) =
+  -- some (ruleset_translation (rs1 ++ [{ matchExpr := m1, action := Action.Return }] ++ rs2))
+    rw [hyp_chain]
+  -- ⊢ Option.map ruleset_translation (some (rs1 ++ [{ matchExpr := m1, action := Action.Return }] ++ rs2)) =
+  -- some (ruleset_translation (rs1 ++ [{ matchExpr := m1, action := Action.Return }] ++ rs2))
+    rfl
+
+  -- since rest is never happens
+  have rest_eval : ruleset_evaluation (translate_ruleset Γ) γ p []
+    {verdict := Verdict.NFT_CONTINUE, destination_chain := none}
+    {verdict := Verdict.NFT_CONTINUE, destination_chain := none} := by
+    exact ruleset_evaluation.skip
+
+  -- ⊢ nf_eval_produces Γ γ p [{ matchExpr := m, action := Action.Call chain }] initial_register ProcessingDecision.undecided
+  unfold nf_eval_produces
+  -- ⊢ ∃ regs_out, ruleset_evaluation (translate_ruleset Γ) γ p (ruleset_translation [{ matchExpr := m, action := Action.Call chain }])
+  -- initial_register regs_out ∧ simulation ProcessingDecision.undecided regs_out
+  use initial_register
+  -- ⊢ ruleset_evaluation (translate_ruleset Γ) γ p (ruleset_translation [{ matchExpr := m, action := Action.Call chain }])
+  -- initial_register initial_register ∧
+  -- simulation ProcessingDecision.undecided initial_register
+  apply And.intro
+  case h.left =>
+    exact ruleset_evaluation.jump rfl h_rule jump_regs jump_dest_chain chain_lookup final_eval rest_eval
+  case h.right =>
+    exact simulation.undecided
+
+theorem call_result_equivalence {A P : Type} (Γ : Ruleset A) (γ : Matcher A P) (p : P)
+  (m : MatchExpr A) (chain : String) (rs : List (Iptables.Rule A)) (t : ProcessingDecision)
+  (hyp_match : matchExpression γ m p = true)
+  (hyp_chain : Γ chain = some rs)
+  (IH_chain : ∀ regs_in, simulation ProcessingDecision.undecided regs_in ->
+    nf_eval_produces Γ γ p rs regs_in t) :
+
+  nf_eval_produces Γ γ p [{ matchExpr := m, action := Action.Call chain }] initial_register t := by
+  -- ⊢ nf_eval_produces Γ γ p [{ matchExpr := m, action := Action.Call chain }] initial_register t
+  unfold nf_eval_produces
+  -- ⊢ ∃ regs_out, ruleset_evaluation (translate_ruleset Γ) γ p (ruleset_translation [{ matchExpr := m, action := Action.Call chain }]) initial_register regs_out ∧
+  -- simulation t regs_out
+  -- the jump rule fires, producing regs1 (verdict=NFT_JUMP, destination = chain)
+  have rule_pf := call_rule_eval Γ γ p m chain hyp_match
+  -- ⊢ ∃ regs_out, ruleset_evaluation (translate_ruleset Γ) γ p (ruleset_translation [{ matchExpr := m, action := Action.Call chain }])
+  -- initial_register regs_out ∧
+  -- simulation t regs_out
+  -- called chain rs evaluates from initial_register to a corresponding to a decision t in nftables
+  have chain_pf : nf_eval_produces Γ γ p rs initial_register t :=
+  IH_chain initial_register simulation.undecided
+  unfold nf_eval_produces at chain_pf
+
+  obtain ⟨regs_out, chain_eval, sim⟩ := chain_pf
+
+  let regs1 := apply_statement (Statement.Jump chain) initial_register
+  have jump_regs : regs1.verdict = Verdict.NFT_JUMP := by rfl
+  have jump_dest : regs1.destination_chain = some chain := by rfl
+  have chain_lookup : (translate_ruleset Γ) chain = some (ruleset_translation rs) := by
+  -- ⊢ translate_ruleset Γ chain = some (ruleset_translation rs)
+    unfold translate_ruleset
+  -- ⊢ Option.map ruleset_translation (Γ chain) = some (ruleset_translation rs)
+    rw [hyp_chain]
+    rfl
+
+  -- ⊢ ∃ regs_out,
+  -- ruleset_evaluation (translate_ruleset Γ) γ p (ruleset_translation [{ matchExpr := m, action := Action.Call chain }])
+  -- initial_register regs_out ∧
+  -- simulation t regs_out
+  cases sim
+  -- case undecided: chain_eval : ruleset_evaluation (translate_ruleset Γ) γ p (ruleset_translation rs) initial_register
+  -- { verdict := Verdict.NFT_CONTINUE, destination_chain := none }
+  -- case allow : ruleset_evaluation (translate_ruleset Γ) γ p (ruleset_translation rs) initial_register
+  -- { verdict := Verdict.NFT_ACCEPT, destination_chain := none }
+  -- case deny:
+  -- chain_eval : ruleset_evaluation (translate_ruleset Γ) γ p (ruleset_translation rs) initial_register
+  -- { verdict := Verdict.NFT_DROP, destination_chain := none }
+  case undecided =>
+    use initial_register
+    apply And.intro
+    -- ⊢ ruleset_evaluation (translate_ruleset Γ) γ p (ruleset_translation [{ matchExpr := m, action := Action.Call chain }])
+    -- initial_register initial_register
+    exact ruleset_evaluation.jump rfl rule_pf jump_regs jump_dest chain_lookup chain_eval ruleset_evaluation.skip
+    exact simulation.undecided
+  case allow =>
+    use {verdict := Verdict.NFT_ACCEPT, destination_chain := none}
+    apply And.intro
+    exact ruleset_evaluation.jump rfl rule_pf jump_regs jump_dest chain_lookup chain_eval ruleset_evaluation.skip
+    exact simulation.allow
+  case deny =>
+    use {verdict := Verdict.NFT_DROP, destination_chain := none}
+    apply And.intro
+    exact ruleset_evaluation.jump rfl rule_pf jump_regs jump_dest chain_lookup chain_eval ruleset_evaluation.skip
+    exact simulation.deny
+
+
+
+-- if iptables evaluates rs from state t to state t',
+-- and the nftables register regs correspond to t (via simulation),
+-- then the translated rules evalouate in nftables from regs
+-- to some regs', that corresponds to t'
+theorem forward_simulation {A P : Type} (Γ : Ruleset A) (γ : Matcher A P) (p : P)
+(rs : List (Iptables.Rule A)) (t t' : ProcessingDecision) (ipt_eval: iptables_bigstep Γ γ p rs t t')
+(regs : Registers) (sm : simulation t regs) :
+∃ regs', ruleset_evaluation (translate_ruleset Γ) γ p (ruleset_translation rs) regs regs' ∧
+simulation t' regs' := by
+--proof by derivation on iptables (ech iptables_bigstep const)
+induction ipt_eval generalizing regs with
+-- in each case, need to connect sm : simulation with the corresponding _equivalence lemma
+
+-- | accept {m} : matchExpression γ m p = true ->
+  -- iptables_bigstep Γ γ p [{ matchExpr := m, action := Action.Accept }]
+  -- ProcessingDecision.undecided (ProcessingDecision.decision FinalDecision.allow)
+
+  /- If the match succeds, a single Accept rule takes iptables
+  from undecided to allow
+  -/
+  | accept =>
+    have regs_eq : regs = initial_register := by
+      cases sm
+      rfl
+    rw[regs_eq]
+    exact accept_equivalence Γ γ p _ ‹_›
+
+  | drop =>
+  /- ⊢ ∃ regs',
+  ruleset_evaluation (translate_ruleset Γ) γ p (ruleset_translation [{ matchExpr := m✝, action := Action.Drop }]) regs
+      regs' ∧
+    simulation (ProcessingDecision.decision Iptables.FinalDecision.deny) regs'
+  -/
+    have regs_eq : regs = initial_register := by
+      cases sm
+      rfl
+
+    rw[regs_eq]
+    exact drop_rej_equivalence Γ γ p _ ‹_›
+
+  | reject =>
+    have regs_eq : regs = initial_register := by
+      cases sm
+      rfl
+
+    rw[regs_eq]
+    exact drop_rej_equivalence Γ γ p _ (by assumption)
+
+  | skip =>
+    exact skip_equivalence Γ γ p _ regs sm
+
+  | log =>
+    have regs_eq : regs = initial_register := by
+      cases sm
+      rfl
+    rw[regs_eq]
+    exact log_equivalence Γ γ p _ (by assumption)
+
+  | empty =>
+    have regs_eq : regs = initial_register := by
+      cases sm
+      rfl
+    rw[regs_eq]
+    exact empty_equivalence Γ γ p _ (by assumption)
+
+  | decision =>
+    exact decision_equivalence Γ γ p _ _ regs sm
+
+  | noMatch =>
+    /- noMatch {m a} : matchExpression γ m p = false →
+    iptables_bigstep Γ γ p [{matchExpr := m, action := a}] undecided undecided
+  -/
+    have regs_eq : regs = initial_register := by
+      cases sm
+      rfl
+    rw[regs_eq]
+    exact noMatch_equivalence Γ γ p _ _ (by assumption)
+
+  | seq =>
+    rename_i rs1 rs2 t1 t2 ev1 ev2 H1 H2
+    have regs_eq : regs = initial_register := by
+      cases sm
+      rfl
+    rw [regs_eq]
+
+    cases t1 with
+    | undecided =>
+      exact seq_equivalence_full Γ γ p rs1 rs2 t2 (fun regs sim => H1 regs sim) (fun regs sim => H2 regs sim) initial_register simulation.undecided
+    | decision d =>
+      /- ⊢ ∃ regs',
+      -- ruleset_evaluation (translate_ruleset Γ) γ p (ruleset_translation (rs1 ++ rs2)) initial_register regs' ∧
+      -- simulation t2 regs' -/
+      have ⟨regs_mid, rs_eval1, sim_mid⟩ := H1 initial_register simulation.undecided
+      cases ev2 with -- pattern matches iptables derivation for rs2
+        | skip =>
+          -- rs1 + [] = rs1
+          simp [List.append_nil]
+          subst regs_eq
+          simp_all only
+        | decision =>
+          have terminal : regs_mid.verdict = Verdict.NFT_ACCEPT ∨ regs_mid.verdict = Verdict.NFT_DROP := by
+            cases sim_mid with
+              | allow =>
+                left
+                rfl
+              | deny =>
+                right
+                rfl
+          /-⊢ ∃ regs',
+          ruleset_evaluation (translate_ruleset Γ) γ p (ruleset_translation (rs1 ++ rs2)) initial_register regs' ∧
+          simulation (ProcessingDecision.decision d) regs'-/
+          use regs_mid
+          /- ⊢ ruleset_evaluation (translate_ruleset Γ) γ p (ruleset_translation (rs1 ++ rs2)) initial_register regs_mid ∧
+          simulation (ProcessingDecision.decision d) regs_mid-/
+          constructor
+          case h.left =>
+            rw [rs_homomorphism]
+            exact ruleset_evaluation_append_terminal rs_eval1 terminal
+          case h.right =>
+            exact sim_mid
+
+  | call_return =>
+    /-| call_return {m chain rs₁ m' rs₂} :
+    matchExpression γ m p = true →            -- (1) call rule matches
+    Γ chain = some (rs₁ ++ [{m', Return}] ++ rs₂) →  -- (2) chain structure
+    matchExpression γ m' p = true →           -- (3) return rule matches
+    iptables_bigstep Γ γ p rs₁ undecided undecided →  -- (4) rs₁ stays undecided
+    iptables_bigstep Γ γ p [{m, Call chain}] undecided undecided
+    -/
+    rename_i m1 chain rs1 m2 rs2 hyp_match1 hyp_chain hyp_match2 eval H1
+    have regs_eq : regs = initial_register := by
+      cases sm
+      rfl
+    rw [regs_eq]
+    have hlpr := call_return_equivalence Γ γ p m1 chain rs1 m2 rs2 hyp_match1 hyp_chain hyp_match2
+      (fun regs_in sim => H1 regs_in sim)
+
+    -- hammer
+    subst regs_eq
+    simp_all only [List.append_assoc, List.cons_append, List.nil_append]
+    exact hlpr
+
+  | call_result =>
+    rename_i m chain rs1 t hyp_match hyp_chain eval1 H1
+    /-
+    | call_result {m chain rs t} :
+    matchExpression γ m p = true →
+    Γ chain = some rs →
+    iptables_bigstep Γ γ p rs undecided t →
+    iptables_bigstep Γ γ p [{ matchExpr := m, action := Action.Call chain }] undecided t
+-/
+  -- set regs = initial_register
+    have regs_eq : regs = initial_register := by
+      cases sm
+      rfl
+    rw [regs_eq]
+    have hlpr := call_result_equivalence Γ γ p _ _ _ _ hyp_match hyp_chain
+      (fun regs_in sim => H1 regs_in sim)
+
+    -- hammer
+    subst regs_eq
+    exact hlpr
